trunk/examples/concurrent/bpl/POPL2023/map-incr-split.bpl
@@ -1,4 +1,9 @@
 //#Safe
+/*
+ * Author: Dominik Klumpp
+ * Date: June 2022
+ */
+
 var A: [int]int;
 var k : int;
 var N : int;
