trunk/examples/concurrent/bpl/POPL2023/min-max-sample-abs-2.bpl
@@ -4,7 +4,7 @@
  * Date: 2022-06-08
  */
  
- // invariant: (i1 <= m \/ array_min <= A[m]) /\ (i2 <= m \/ A[m] <= array_max)
+// invariant: (i1 <= m \/ array_min <= A[m]) /\ (i2 <= m \/ A[m] <= array_max)
 
 var A : [int]int;
 var N : int;
