trunk/examples/concurrent/bpl/POPL2023/min-max-sample-with_locks.bpl
@@ -1,9 +1,8 @@
 //#Safe
 /*
- * Benchmark where (variable) abstraction is essential:
+ * Benchmark for (variable) abstraction:
  *
- * To prove the property, loop-lockstep alignment between computeMin and computeMax is crucial.
- * However, while these threads commute concretely, they only commute abstractly against the sample thread.
+ * While computeMin and computeMax commute concretely, they only commute abstractly against the sample thread.
  *
  * However, because computeMin and computeMax are disjoint, they in fact also commute under lightweight-abstract.
  *
