trunk/examples/concurrent/bpl/POPL2023/motivating-slowitp.bpl
@@ -1,20 +1,7 @@
 //#Safe
 /*
- * Idea: thread1 and thread2 full commute up to concrete-SMT; B can be abstracted away so that thread2 also commutes abstract-lightweight against thread3.
- *
- * Principle: thread1 performs map(A, f)
- *            thread2 performs aggr(A, B)
- *            thread3 performs update(B)
- *            such that map(_, f) and aggr(_, B) commute concretely (SMT);
-              while aggr(A, _) and update(_) do NOT commute concretely but B is irrelevant for the spec.
-
-              other instances:
-              f      aggr            update     property
-              ---------------------------------------------------------
-              relU   max_pos_index   :=k        A[m]>0 ==> result >= m
-              abs    sum_abs         :=0        result >= |A[m]|
-              abs    cnt_zeroes      :=0        ...
-              abs    max_zero_index  :=0        ...
+ * Author: Dominik Klumpp
+ * Date: June 2022
  */
 
 var A, B : [int]int;
