trunk/examples/concurrent/bpl/POPL2023/sumsumbank.bpl
@@ -1,4 +1,8 @@
 //#Safe
+/*
+ * Author: Dominik Klumpp
+ * Date: June 2022
+ */
 
 var A, B : [int]int;
 var N : int;
